filteration

Foundation/Modal/Kripke/Filteration.lean
@@ -1,24 +1,31 @@
-import Foundation.Logic.Kripke.Closure
-import Foundation.Modal.Kripke.Completeness
 import Foundation.Modal.Kripke.Geach
+import Foundation.Modal.Kripke.Closure
 
 universe u v
 
 namespace LO.Modal
 
-variable {α : Type u} -- [DecidableEq α] [Inhabited α]
-
 namespace Kripke
 
-open LO.Kripke
 open Formula (atom)
 open Formula.Kripke
 
 section
 
-def filterEquiv (M : Kripke.Model α) (T : Theory α) [T.SubformulaClosed] (x y : M.World) := ∀ φ, (_ : φ ∈ T := by trivial) → x ⊧ φ ↔ y ⊧ φ
+abbrev ReflexiveSymmetricFiniteFrameClass : FiniteFrameClass := { F | Reflexive F.Rel ∧ Symmetric F.Rel }
 
-variable (M : Kripke.Model α) (T : Theory α) [T.SubformulaClosed]
+abbrev ReflexiveTransitiveFiniteFrameClass : FiniteFrameClass := { F | Reflexive F.Rel ∧ Transitive F.Rel }
+
+abbrev ReflexiveTransitiveSymmetricFiniteFrameClass : FiniteFrameClass := { F | Reflexive F.Rel ∧ Transitive F.Rel ∧ Symmetric F.Rel }
+
+end
+
+
+section
+
+def filterEquiv (M : Kripke.Model) (T : Theory ℕ) [T.SubformulaClosed] (x y : M.World) := ∀ φ, (_ : φ ∈ T := by trivial) → x ⊧ φ ↔ y ⊧ φ
+
+variable (M : Kripke.Model) (T : Theory ℕ) [T.SubformulaClosed]
 
 lemma filterEquiv.equivalence : Equivalence (filterEquiv M T) where
   refl := by intro x φ _; rfl;
@@ -57,11 +64,11 @@ lemma FilterEqvQuotient.finite (T_finite : T.Finite) : Finite (FilterEqvQuotient
       exact this φ hp hpy |>.2;
   exact Finite.of_injective f hf
 
-instance : Nonempty (FilterEqvQuotient M T) := ⟨⟦﹫⟧⟩
+instance : Nonempty (FilterEqvQuotient M T) := ⟨⟦M.toFrame.world_nonempty.some⟧⟩
 
-class FilterOf (FM : Model α) (M : Model α) (T : Theory α) [T.SubformulaClosed] where
+class FilterOf (FM : Model) (M : Model) (T : Theory ℕ) [T.SubformulaClosed] : Prop where
   def_world : FM.World = FilterEqvQuotient M T := by rfl
-  def_rel₁ : ∀ {x y : M.Frame}, x ≺ y → Frame.Rel' (cast def_world.symm ⟦x⟧) (cast def_world.symm ⟦y⟧) := by tauto;
+  def_rel₁ : ∀ {x y : M.toFrame}, x ≺ y → Frame.Rel' (cast def_world.symm ⟦x⟧) (cast def_world.symm ⟦y⟧) := by tauto;
   def_box : ∀ {Qx Qy : FM.World}, Qx ≺ Qy → Quotient.lift₂ (λ x y => ∀ φ, □φ ∈ T → (x ⊧ □φ → y ⊧ φ)) (by
     intro x₁ y₁ x₂ y₂ hx hy;
     simp;
@@ -70,7 +77,7 @@ class FilterOf (FM : Model α) (M : Model α) (T : Theory α) [T.SubformulaClose
     . intro h φ hp sp₁; exact hy φ |>.mpr $ h φ hp $ hx (□φ) hp |>.mp sp₁;
   ) (cast def_world Qx) (cast def_world Qy)
   def_valuation Qx a : (ha : (atom a) ∈ T := by trivial) →
-    FM.Valuation Qx a ↔ Quotient.lift (λ x => M.Valuation x a) (by
+    FM Qx a ↔ Quotient.lift (λ x => M x a) (by
       simp; intro x y h;
       constructor;
       . intro hx; exact h a ha |>.mp hx;
@@ -79,11 +86,27 @@ class FilterOf (FM : Model α) (M : Model α) (T : Theory α) [T.SubformulaClose
 
 attribute [simp] FilterOf.def_world
 
-namespace FilterationModel
+section
 
-end FilterationModel
+variable {M T}
 
-abbrev StandardFilterationValuation (Qx : FilterEqvQuotient M T) (a : α) := (ha : (atom a) ∈ T) → Quotient.lift (λ x => M.Valuation x a) (by
+lemma reflexive_filterOf_of_reflexive (h_filter : FilterOf FM M T) (hRefl : Reflexive M.toFrame) : Reflexive FM.Rel := by
+  intro Qx;
+  obtain ⟨x, hx⟩ := Quotient.exists_rep (cast (h_filter.def_world) Qx);
+  convert h_filter.def_rel₁ $ hRefl x <;> simp_all;
+
+lemma serial_filterOf_of_serial (h_filter : FilterOf FM M T) (hSerial : Serial M.toFrame) : Serial FM.Rel := by
+  intro Qx;
+  obtain ⟨x, hx⟩ := Quotient.exists_rep (cast (h_filter.def_world) Qx);
+  obtain ⟨y, Rxy⟩ := hSerial x;
+  use (cast (h_filter.def_world.symm) ⟦y⟧);
+  convert h_filter.def_rel₁ $ Rxy;
+  simp_all;
+
+end
+
+
+abbrev standardFilterationValuation (Qx : FilterEqvQuotient M T) (a : ℕ) := (ha : (atom a) ∈ T) → Quotient.lift (λ x => M x a) (by
   simp; intro x y h;
   constructor;
   . intro hx; exact h a ha |>.mp hx;
@@ -91,21 +114,7 @@ abbrev StandardFilterationValuation (Qx : FilterEqvQuotient M T) (a : α) := (ha
 ) Qx
 
 
-abbrev FinestFilterationFrame (M : Model α) (T : Theory α) [T.SubformulaClosed] : Kripke.Frame where
-  World := FilterEqvQuotient M T
-  Rel Qx Qy := ∃ x y, Qx = ⟦x⟧ ∧ Qy = ⟦y⟧ ∧ x ≺ y
-
-abbrev FinestFilterationModel (M : Model α) (T : Theory α) [T.SubformulaClosed] : Kripke.Model α where
-  Frame := FinestFilterationFrame M T
-  Valuation := StandardFilterationValuation M T
-
-instance FinestFilterationModel.filterOf {M} {T : Theory α} [T.SubformulaClosed] : FilterOf (FinestFilterationModel M T) M T where
-  def_box := by
-    intro Qx Qy rQxQy;
-    obtain ⟨x, y, rfl, rfl, hxy⟩ := rQxQy;
-    simp_all [Satisfies];
-
-abbrev CoarsestFilterationFrame (M : Model α) (T : Theory α) [T.SubformulaClosed] : Kripke.Frame where
+abbrev coarsestFilterationFrame (M : Model) (T : Theory ℕ) [T.SubformulaClosed] : Kripke.Frame where
   World := FilterEqvQuotient M T
   Rel Qx Qy :=
     Quotient.lift₂ (λ x y => ∀ φ, □φ ∈ T → (x ⊧ □φ → y ⊧ φ)) (by
@@ -116,47 +125,94 @@ abbrev CoarsestFilterationFrame (M : Model α) (T : Theory α) [T.SubformulaClos
       . intro h φ hp sp₁; exact hy φ |>.mpr $ h φ hp $ hx (□φ) hp |>.mp sp₁;
     ) Qx Qy
 
-abbrev CoarsestFilterationModel (M : Model α) (T : Theory α) [T.SubformulaClosed] : Kripke.Model α where
-  Frame := CoarsestFilterationFrame M T
-  Valuation := StandardFilterationValuation M T
+abbrev coarsestFilterationModel (M : Model) (T : Theory ℕ) [T.SubformulaClosed] : Kripke.Model where
+  toFrame := coarsestFilterationFrame M T
+  Val := standardFilterationValuation M T
 
-instance CoarsestFilterationModel.filterOf {M} {T : Theory α} [T.SubformulaClosed] : FilterOf (CoarsestFilterationModel M T) M T where
+instance coarsestFilterationModel.filterOf {M} {T : Theory ℕ} [T.SubformulaClosed] : FilterOf (coarsestFilterationModel M T) M T where
   def_box := by tauto
 
-section
 
-variable {M} {T : Theory α} [T.SubformulaClosed] {FM : Kripke.Model α}
+abbrev finestFilterationFrame (M : Model) (T : Theory ℕ) [T.SubformulaClosed] : Kripke.Frame where
+  World := FilterEqvQuotient M T
+  Rel Qx Qy := ∃ x y, Qx = ⟦x⟧ ∧ Qy = ⟦y⟧ ∧ x ≺ y
 
-lemma reflexive_filteration_model (h_filter : FilterOf FM M T) (hRefl : Reflexive M.Frame) : Reflexive FM.Frame := by
-  intro Qx;
-  obtain ⟨x, hx⟩ := Quotient.exists_rep (cast (h_filter.def_world) Qx);
-  convert h_filter.def_rel₁ $ hRefl x <;> simp_all;
+abbrev finestFilterationModel (M : Model) (T : Theory ℕ) [T.SubformulaClosed] : Kripke.Model where
+  toFrame := finestFilterationFrame M T
+  Val := standardFilterationValuation M T
 
-lemma serial_filteration_model (h_filter : FilterOf FM M T) (hSerial : Serial M.Frame) : Serial FM.Frame := by
-  intro Qx;
-  obtain ⟨x, hx⟩ := Quotient.exists_rep (cast (h_filter.def_world) Qx);
-  obtain ⟨y, Rxy⟩ := hSerial x;
-  use (cast (h_filter.def_world.symm) ⟦y⟧);
-  convert h_filter.def_rel₁ $ Rxy;
-  simp_all;
+namespace finestFilterationModel
 
-lemma symmetric_finest_filteration_model (hSymm : Symmetric M.Frame) : Symmetric (FinestFilterationModel M T).Frame := by
+variable {M T}
+
+instance filterOf [T.SubformulaClosed] : FilterOf (finestFilterationModel M T) M T where
+  def_box := by
+    intro Qx Qy rQxQy;
+    obtain ⟨x, y, rfl, rfl, _⟩ := rQxQy;
+    simp_all [Satisfies];
+
+lemma symmetric_of_symmetric (hSymm : Symmetric M.toFrame) : Symmetric (finestFilterationModel M T).Rel := by
   intro Qx Qy RQxQy;
   obtain ⟨x, y, hx, hy, h⟩ := RQxQy; subst_vars;
   use y, x; simp;
   exact hSymm h;
 
-end
+end finestFilterationModel
+
+
+abbrev finestFilterationTransitiveClosureModel (M : Model) (T : Theory ℕ) [T.SubformulaClosed] : Kripke.Model where
+  toFrame := (finestFilterationFrame M T)^+
+  Val := standardFilterationValuation M T
+
+namespace finestFilterationTransitiveClosureModel
+
+variable {M T}
+
+instance filterOf (M_trans : Transitive M.Rel) : FilterOf (finestFilterationTransitiveClosureModel M T) M T where
+  def_rel₁ := by
+    intro x y hxy;
+    apply Frame.TransitiveClosure.single;
+    tauto;
+  def_box := by
+    intro Qx Qy RQxQy;
+    induction RQxQy using Relation.TransGen.head_induction_on with
+    | base rxy =>
+      obtain ⟨x, y, rfl, rfl, rxy⟩ := rxy;
+      intro φ _ hpx;
+      exact hpx _ rxy;
+    | ih ha hxy hyz =>
+      obtain ⟨x, y, rfl, rfl, rxy⟩ := ha;
+      obtain ⟨w, z, _, rfl, _⟩ := hxy;
+      . intro φ hp hpx;
+        apply hyz φ hp;
+        intro v ryv;
+        exact hpx _ (M_trans rxy ryv);
+      . rename_i h;
+        obtain ⟨w, z, rfl, rfl, _⟩ := h;
+        intro φ hp hpx;
+        apply hyz φ hp;
+        intro v ryv;
+        exact hpx _ (M_trans rxy ryv);
+
+lemma transitive : Transitive (finestFilterationTransitiveClosureModel M T).Rel := Frame.TransitiveClosure.rel_transitive
+
+lemma symmetric_of_symmetric (M_symm : Symmetric M.Rel) : Symmetric (finestFilterationTransitiveClosureModel M T).Rel :=
+  Frame.TransitiveClosure.rel_symmetric $ finestFilterationModel.symmetric_of_symmetric M_symm
+
+lemma reflexive_of_transitive_reflexive (M_trans : Transitive M.Rel) (M_refl : Reflexive M.Rel) : Reflexive (finestFilterationTransitiveClosureModel M T).Rel := by
+  exact reflexive_filterOf_of_reflexive (filterOf M_trans) M_refl;
+
+end finestFilterationTransitiveClosureModel
 
 end
 
 
 section
 
-variable {M : Model α} {T : Theory α} [T.SubformulaClosed]
-         (FM : Model α) (filterOf : FilterOf FM M T)
+variable {M : Model} {T : Theory ℕ} [T.SubformulaClosed]
+         (FM : Model) (filterOf : FilterOf FM M T)
 
-theorem filteration {x : M.World} {φ : Formula α} (hs : φ ∈ T := by trivial) : x ⊧ φ ↔ (cast (filterOf.def_world.symm) ⟦x⟧) ⊧ φ := by
+theorem filteration {x : M.World} {φ : Formula ℕ} (hs : φ ∈ T := by trivial) : x ⊧ φ ↔ (cast (filterOf.def_world.symm) ⟦x⟧) ⊧ φ := by
   induction φ using Formula.rec' generalizing x with
   | hatom a =>
     have := filterOf.def_valuation (cast filterOf.def_world.symm ⟦x⟧) a;
@@ -180,144 +236,115 @@ theorem filteration {x : M.World} {φ : Formula α} (hs : φ ∈ T := by trivial
 
 end
 
-instance K_finite_complete [DecidableEq α] : Complete (Hilbert.K α) (AllFrameClass.{u}ꟳ#α) := ⟨by
+end Kripke
+
+
+namespace Hilbert
+
+open Modal.Kripke
+open Hilbert.Kripke
+
+instance K.Kripke.finite_complete : Complete (Hilbert.K ℕ) (AllFiniteFrameClass) := ⟨by
   intro φ hp;
-  apply K_complete.complete;
+  apply Hilbert.K.Kripke.complete.complete;
   intro F _ V x;
-  let M : Kripke.Model α := ⟨F, V⟩;
-  let FM := CoarsestFilterationModel M ↑φ.subformulae;
+  let M : Kripke.Model := ⟨F, V⟩;
+  let FM := coarsestFilterationModel M ↑φ.subformulae;
 
-  apply filteration FM (CoarsestFilterationModel.filterOf) (by aesop) |>.mpr;
-  apply hp (by
-    suffices Finite (FilterEqvQuotient M φ.subformulae) by simp; use ⟨FM.Frame⟩;
-    apply FilterEqvQuotient.finite;
-    simp;
-  ) FM.Valuation
-⟩
-
-instance  [DecidableEq α] : FiniteFrameProperty (Hilbert.K α) AllFrameClass where
-
-
-instance KTB_finite_complete [DecidableEq α] [Inhabited α] : Complete (Hilbert.KTB α) (ReflexiveSymmetricFrameClass.{u}ꟳ#α) := ⟨by
-  intro φ hp;
-  apply KTB_complete.complete;
-  intro F ⟨F_refl, F_symm⟩ V x;
-  let M : Kripke.Model α := ⟨F, V⟩;
-  let FM := FinestFilterationModel M φ.subformulae;
-  apply filteration FM (FinestFilterationModel.filterOf) (by aesop) |>.mpr;
+  apply filteration FM (coarsestFilterationModel.filterOf) (by aesop) |>.mpr;
   apply hp (by
     suffices Finite (FilterEqvQuotient M φ.subformulae) by
-      use ⟨FM.Frame⟩;
+      simp [AllFiniteFrameClass, FiniteFrameClass.toFrameClass];
+      use ⟨FM.toFrame⟩;
+    apply FilterEqvQuotient.finite;
+    simp;
+  ) FM.Val
+⟩
+
+instance K.Kripke.ffp : FiniteFrameProperty (Hilbert.K ℕ) AllFiniteFrameClass where
+  complete := K.Kripke.finite_complete
+  sound := Kripke.instFiniteSound_of_instSound (C := AllFrameClass) (FC := AllFiniteFrameClass) rfl
+
+
+instance KTB.Kripke.finite_complete : Complete (Hilbert.KTB ℕ) (ReflexiveSymmetricFiniteFrameClass) := ⟨by
+  intro φ hp;
+  apply Hilbert.KTB.Kripke.complete.complete;
+  intro F ⟨F_refl, F_symm⟩ V x;
+  let M : Kripke.Model := ⟨F, V⟩;
+  let FM := finestFilterationModel M φ.subformulae;
+  apply filteration FM (finestFilterationModel.filterOf) (by aesop) |>.mpr;
+  apply hp (by
+    suffices Finite (FilterEqvQuotient M φ.subformulae) by
+      simp [ReflexiveSymmetricFiniteFrameClass, FiniteFrameClass.toFrameClass];
+      use ⟨FM.toFrame⟩;
       refine ⟨⟨?_, ?_⟩, ?_⟩;
-      . apply reflexive_filteration_model (FinestFilterationModel.filterOf);
+      . apply reflexive_filterOf_of_reflexive (finestFilterationModel.filterOf);
         exact F_refl;
-      . apply symmetric_finest_filteration_model;
+      . apply finestFilterationModel.symmetric_of_symmetric;
         exact F_symm;
       . rfl;
     apply FilterEqvQuotient.finite;
     simp;
-  ) FM.Valuation
+  ) FM.Val
 ⟩
 
-instance [DecidableEq α] [Inhabited α] : FiniteFrameProperty (Hilbert.KTB α) ReflexiveSymmetricFrameClass where
+instance KTB.Kripke.ffp : FiniteFrameProperty (Hilbert.KTB ℕ) ReflexiveSymmetricFiniteFrameClass where
+  complete := KTB.Kripke.finite_complete
+  sound := Kripke.instFiniteSound_of_instSound (C := ReflexiveSymmetricFrameClass) (FC := ReflexiveSymmetricFiniteFrameClass) rfl
 
-section
 
-open Kripke.Frame (TransitiveClosure)
-
-variable {M : Model α} {T : Theory α} [T.SubformulaClosed]
-
-abbrev FinestFilterationTransitiveClosureModel (M : Model α) (T : Theory α) [T.SubformulaClosed] : Kripke.Model α where
-  Frame := (FinestFilterationFrame M T)^+
-  Valuation := StandardFilterationValuation M T
-
-namespace FinestFilterationTransitiveClosureModel
-
-instance filterOf (M_trans : Transitive M.Frame) : FilterOf (FinestFilterationTransitiveClosureModel M T) M T where
-  def_rel₁ := by
-    intro x y hxy;
-    apply TransitiveClosure.single;
-    tauto;
-  def_box := by
-    intro Qx Qy RQxQy;
-    induction RQxQy using Relation.TransGen.head_induction_on with
-    | base rxy =>
-      obtain ⟨x, y, rfl, rfl, rxy⟩ := rxy;
-      intro φ _ hpx;
-      exact hpx _ rxy;
-    | ih ha hxy hyz =>
-      obtain ⟨x, y, rfl, rfl, rxy⟩ := ha;
-      obtain ⟨w, z, _, rfl, _⟩ := hxy;
-      . intro φ hp hpx;
-        apply hyz φ hp;
-        intro v ryv;
-        exact hpx _ (M_trans rxy ryv);
-      . rename_i h;
-        obtain ⟨w, z, rfl, rfl, _⟩ := h;
-        intro φ hp hpx;
-        apply hyz φ hp;
-        intro v ryv;
-        exact hpx _ (M_trans rxy ryv);
-
-lemma rel_transitive : Transitive (FinestFilterationTransitiveClosureModel M T).Frame := Frame.TransitiveClosure.rel_transitive
-
-lemma rel_symmetric (M_symm : Symmetric M.Frame) : Symmetric (FinestFilterationTransitiveClosureModel M T).Frame :=
-  Frame.TransitiveClosure.rel_symmetric $ symmetric_finest_filteration_model M_symm
-
-lemma rel_reflexive (M_trans : Transitive M.Frame) (M_refl : Reflexive M.Frame) : Reflexive (FinestFilterationTransitiveClosureModel M T).Frame := by
-  exact reflexive_filteration_model (filterOf M_trans) M_refl;
-
-end FinestFilterationTransitiveClosureModel
-
-end
-
-open FinestFilterationTransitiveClosureModel in
-instance S4_finite_complete [Inhabited α] [DecidableEq α] : Complete (Hilbert.S4 α) (PreorderFrameClass.{u}ꟳ#α) := ⟨by
+open finestFilterationTransitiveClosureModel in
+instance S4.Kripke.finite_complete : Complete (Hilbert.S4 ℕ) (ReflexiveTransitiveFiniteFrameClass) := ⟨by
   intro φ hp;
-  apply S4_complete.complete;
+  apply Hilbert.S4.Kripke.complete.complete;
   intro F ⟨F_refl, F_trans⟩ V x;
-  let M : Kripke.Model α := ⟨F, V⟩;
-  let FM := FinestFilterationTransitiveClosureModel M φ.subformulae;
-  apply @filteration α M φ.subformulae _ FM ?filterOf x φ (by simp) |>.mpr;
+  let M : Kripke.Model := ⟨F, V⟩;
+  let FM := finestFilterationTransitiveClosureModel M φ.subformulae;
+  apply @filteration M φ.subformulae _ FM ?filterOf x φ (by simp) |>.mpr;
   apply hp (by
     suffices Finite (FilterEqvQuotient M φ.subformulae) by
-      use ⟨FM.Frame⟩;
-      refine ⟨⟨?_, rel_transitive⟩, rfl⟩;
-      . exact rel_reflexive (by apply F_trans) F_refl;
+      simp [ReflexiveSymmetricFiniteFrameClass, FiniteFrameClass.toFrameClass];
+      use ⟨FM.toFrame⟩;
+      refine ⟨⟨?_, transitive⟩, rfl⟩;
+      . exact reflexive_of_transitive_reflexive (by apply F_trans) F_refl;
     apply FilterEqvQuotient.finite;
     simp;
-  ) FM.Valuation;
-  . apply FinestFilterationTransitiveClosureModel.filterOf;
+  ) FM.Val;
+  . apply finestFilterationTransitiveClosureModel.filterOf;
     exact F_trans;
 ⟩
 
-instance [Inhabited α] [DecidableEq α] : FiniteFrameProperty (Hilbert.S4 α) PreorderFrameClass where
+instance S4.Kripke.ffp : FiniteFrameProperty (Hilbert.S4 ℕ) ReflexiveTransitiveFiniteFrameClass where
+  complete := S4.Kripke.finite_complete
+  sound := Kripke.instFiniteSound_of_instSound (C := ReflexiveTransitiveFrameClass) (FC := ReflexiveTransitiveFiniteFrameClass) rfl
 
 
-open FinestFilterationTransitiveClosureModel in
-instance KT4B_finite_complete [Inhabited α] [DecidableEq α] : Complete (Hilbert.KT4B α) (EquivalenceFrameClass.{u}ꟳ#α) := ⟨by
+open finestFilterationTransitiveClosureModel in
+instance KT4B.Kripke.finite_complete : Complete (Hilbert.KT4B ℕ) (ReflexiveTransitiveSymmetricFiniteFrameClass) := ⟨by
   intro φ hp;
-  apply KT4B_complete.complete;
+  apply Hilbert.KT4B.Kripke.complete.complete;
   intro F ⟨F_refl, F_trans, F_symm⟩ V x;
-  let M : Kripke.Model α := ⟨F, V⟩;
-  let FM := FinestFilterationTransitiveClosureModel M φ.subformulae;
-  apply @filteration α M φ.subformulae _ FM ?filterOf x φ (by simp) |>.mpr;
+  let M : Kripke.Model := ⟨F, V⟩;
+  let FM := finestFilterationTransitiveClosureModel M φ.subformulae;
+  apply @filteration M φ.subformulae _ FM ?filterOf x φ (by simp) |>.mpr;
   apply hp (by
     suffices Finite (FilterEqvQuotient M φ.subformulae) by
-      use ⟨FM.Frame⟩;
-      refine ⟨⟨?refl, rel_transitive, ?symm⟩, rfl⟩;
-      . exact rel_reflexive (by apply F_trans) F_refl;
-      . exact rel_symmetric F_symm;
+      simp [ReflexiveSymmetricFiniteFrameClass, FiniteFrameClass.toFrameClass];
+      use ⟨FM.toFrame⟩;
+      refine ⟨⟨?refl, transitive, ?symm⟩, rfl⟩;
+      . exact reflexive_of_transitive_reflexive (by apply F_trans) F_refl;
+      . exact symmetric_of_symmetric F_symm;
     apply FilterEqvQuotient.finite;
     simp;
-  ) FM.Valuation;
-  . apply FinestFilterationTransitiveClosureModel.filterOf
+  ) FM.Val;
+  . apply finestFilterationTransitiveClosureModel.filterOf
     exact F_trans;
 ⟩
 
-instance [Inhabited α] [DecidableEq α] : FiniteFrameProperty (Hilbert.KT4B α) EquivalenceFrameClass where
--- MEMO: `𝐒𝟓 =ₛ 𝐊𝐓𝟒𝐁`だから決定可能性という面では`𝐒𝟓`も決定可能．
+instance KT4B.Kripke.ffp : FiniteFrameProperty (Hilbert.KT4B ℕ) ReflexiveTransitiveSymmetricFiniteFrameClass where
+  complete := KT4B.Kripke.finite_complete
+  sound := Kripke.instFiniteSound_of_instSound (C := ReflexiveTransitiveSymmetricFrameClass) (FC := ReflexiveTransitiveSymmetricFiniteFrameClass) rfl
 
-end Kripke
+end Hilbert
 
 end LO.Modal
